pushing refactoring through interop/new ...almost there

vale/code/arch/x64/interop/new/Vale.AsLowStar.MemoryHelpers.fst
@@ -1,45 +1,20 @@
 module Vale.AsLowStar.MemoryHelpers
-
+open X64.MemoryAdapters
 open Interop.Base
 module B = LowStar.Buffer
-module BS = X64.Bytes_Semantics_s
 module BV = LowStar.BufferView
-module HS = FStar.HyperStack
 module ME = X64.Memory
-module MES = X64.Memory_Sems
-module TS = X64.Taint_Semantics_s
-module MS = X64.Machine_s
-module IA = Interop.Assumptions
-module IM = Interop.Mem
-module V = X64.Vale.Decls
-module VS = X64.Vale.State
-module IX64 = Interop.X64
 module VSig = Vale.AsLowStar.ValeSig
-module LSig = Vale.AsLowStar.LowStarSig
-module SL = X64.Vale.StateLemmas
-module VL = X64.Vale.Lemmas
-module ST = FStar.HyperStack.ST
 
 friend X64.Memory
 friend X64.Memory_Sems
 friend X64.Vale.Decls
 friend X64.Vale.StateLemmas
-open Interop.Adapters
 
-let as_vale_buffer_len (#t:ME.typ) (x:lowstar_buffer t)
-   = admit()
+let as_vale_buffer_len (#t:base_typ) (x:buf_t t)
+   = BV.length_eq (BV.mk_buffer_view (as_vale_buffer x) (ME.uint_view t))
 
-let down_mem_unify () : Lemma (IM.down_mem == Interop.down_mem) = 
-     admit() // TODO: We should only have one def for down_mem
-
-let mem_reveal (mem:ME.mem) : Lemma 
-  (hs_of_mem mem == mem.ME.hs /\ ptrs_of_mem mem == mem.ME.ptrs)
-  = admit() // TODO: Will be provable with an implementation for Interop.Adapters
-
-let state_eq_down_mem (va_s1:V.va_state) (s1:_)
-  = down_mem_unify();
-    mem_reveal va_s1.VS.mem;
-    assume (va_s1.VS.mem.ME.addrs == IA.addrs) //TODO: Needs a stronger invariant on mem.addrs
+let state_eq_down_mem (va_s1:V.va_state) (s1:_) = ()
 
 let rec loc_eq (args:list arg)
   : Lemma (VSig.mloc_modified_args args == loc_modified_args args)
@@ -47,47 +22,20 @@ let rec loc_eq (args:list arg)
     | [] -> ()
     | hd :: tl -> loc_eq tl
 
-let relate_modifies (args:list arg) (m0 m1 : ME.mem)
-  = loc_eq args;
-    mem_reveal m0;
-    mem_reveal m1
-
-let mk_mem_addrs_reveal (args:list arg) (h0:mem_roots args) : Lemma
-  (let mem = mk_mem args h0 in
-   IA.addrs == mem.ME.addrs) =
-   admit() // TODO: Will be provable with an implementation for Interop.Adapters
-
-let reveal_readable (#t:_) (x:lowstar_buffer t) (s:ME.mem)
-  = mem_reveal s
-
-let readable_live (#t:_) (x:lowstar_buffer t) (s:ME.mem)
-  = mem_reveal s
-
-let buffer_readable_reveal #n bt x args h0 stack =
-  let mem = mk_mem (arg_of_lb stack::args) h0 in
-  mk_mem_injective (arg_of_lb stack::args) h0;
-  mem_reveal mem
-
-let get_heap_mk_mem_reveal #n args h0 stack =
-  mk_mem_injective (arg_of_lb stack::args) h0;
-  down_mem_unify ();
-  mk_mem_addrs_reveal (arg_of_lb stack::args) h0;
-  mem_reveal (mk_mem (arg_of_lb stack::args) h0)
-
-let buffer_as_seq_reveal #n t x args h0 stack =
-  assume (t <> ME.TUInt128); // TODO: TUInt128
-  mk_mem_injective (arg_of_lb stack::args) h0;
-  mem_reveal (mk_mem (arg_of_lb stack::args) h0)
-  
-let buffer_as_seq_reveal2 t x va_s =
-  assume (t <> ME.TUInt128); // TODO: TUInt128
-  let mem = va_s.VS.mem in
-  mem_reveal mem
-  
-let buffer_addr_reveal t x args h0 =
-  mk_mem_addrs_reveal args h0;
-  mem_reveal (mk_mem args h0)
-
+let relate_modifies (args:list arg) (m0 m1 : ME.mem) = loc_eq args
+let reveal_readable (#t:_) (x:buf_t t) (s:ME.mem) = ()
+let readable_live (#t:_) (x:buf_t t) (s:ME.mem) = ()
+let buffer_readable_reveal #n bt x args h0 stack = ()
+let get_heap_mk_mem_reveal #n args h0 stack = ()
+let buffer_as_seq_reveal #n t x args h0 stack = ()
+let buffer_as_seq_reveal2 t x va_s = ()
+let buffer_addr_reveal t x args h0 = ()
 let fuel_eq = ()
-
 let decls_eval_code_reveal c va_s0 va_s1 f = ()
+let as_vale_buffer_disjoint (#t1 #t2:base_typ) (x:buf_t t1) (y:buf_t t2) = ()
+
+module IB=Interop.Base
+module MS=X64.Machine_s
+let valid_memtaint (mem:ME.mem) (ps:list b8{IB.list_disjoint_or_eq ps}) (ts:b8 -> GTot MS.taint)
+  : Lemma (ME.valid_taint_bufs mem (IB.create_memtaint mem ps ts) ps ts)
+  = ME.valid_memtaint mem ps ts
