vale/code/arch/x64/interop/new/Vale.AsLowStar.MemoryHelpers.fsti
@@ -1,5 +1,5 @@
 module Vale.AsLowStar.MemoryHelpers
-
+open X64.MemoryAdapters
 open Interop.Base
 module B = LowStar.Buffer
 module BS = X64.Bytes_Semantics_s
@@ -10,7 +10,6 @@ module MES = X64.Memory_Sems
 module TS = X64.Taint_Semantics_s
 module MS = X64.Machine_s
 module IA = Interop.Assumptions
-module IM = Interop.Mem
 module V = X64.Vale.Decls
 module VS = X64.Vale.State
 module IX64 = Interop.X64
@@ -19,9 +18,9 @@ module LSig = Vale.AsLowStar.LowStarSig
 module SL = X64.Vale.StateLemmas
 module VL = X64.Vale.Lemmas
 module ST = FStar.HyperStack.ST
+module I = Interop
 
-
-val as_vale_buffer_len (#t:ME.typ) (x:lowstar_buffer t)
+val as_vale_buffer_len (#t:base_typ) (x:buf_t t)
    : Lemma (V.buffer_length (as_vale_buffer x) == B.length x / view_n t)
            [SMTPat (V.buffer_length (as_vale_buffer x))]
 
@@ -31,12 +30,7 @@ val state_eq_down_mem (va_s1:V.va_state) (s1:_)
         VL.state_eq_opt (Some (SL.state_to_S va_s1)) 
                         (Some s1))
       (ensures (
-         let h1 = (Interop.Adapters.hs_of_mem va_s1.VS.mem) in
-         let final_mem = va_s1.VS.mem in
-         IM.down_mem h1
-                     IA.addrs
-                     (Interop.Adapters.ptrs_of_mem final_mem) ==
-         s1.TS.state.BS.mem))
+         I.down_mem (as_mem va_s1.VS.mem) == s1.TS.state.BS.mem))
 
 val relate_modifies (args:list arg) (m0 m1 : ME.mem)
   : Lemma 
@@ -44,71 +38,69 @@ val relate_modifies (args:list arg) (m0 m1 : ME.mem)
         ME.modifies (VSig.mloc_modified_args args) m0 m1)
       (ensures 
         B.modifies (loc_modified_args args) 
-                   (Interop.Adapters.hs_of_mem m0)
-                   (Interop.Adapters.hs_of_mem m1))
+                   (hs_of_mem (as_mem m0))
+                   (hs_of_mem (as_mem m1)))
 
-val reveal_readable (#t:_) (x:lowstar_buffer t) (s:ME.mem)
+val reveal_readable (#t:_) (x:buf_t t) (s:ME.mem)
   : Lemma 
-      ( List.memP x (Interop.Adapters.ptrs_of_mem s) <==>
+      ( List.memP x (ptrs_of_mem (as_mem s)) <==>
         ME.buffer_readable s (as_vale_buffer x) )
 
-val readable_live (#t:_) (x:lowstar_buffer t) (s:ME.mem)
+val readable_live (#t:_) (x:buf_t t) (s:ME.mem)
   : Lemma 
       ( ME.buffer_readable s (as_vale_buffer x) ==>
-        B.live (Interop.Adapters.hs_of_mem s) x)
+        B.live (hs_of_mem (as_mem s)) x)
 
 val buffer_readable_reveal 
   (#n:_)
-  (bt:ME.base_typ)
-  (x:lowstar_buffer (ME.TBase bt)) 
+  (bt:base_typ)
+  (x:buf_t bt)
   (args:IX64.arity_ok arg)
   (h0:HS.mem)
   (stack:IX64.stack_buffer n{mem_roots_p h0 (arg_of_sb stack::args)}) : Lemma (
-    let mem = Interop.Adapters.mk_mem (arg_of_sb stack::args) h0 in
-    ME.buffer_readable mem (as_vale_buffer #(ME.TBase bt) x) <==>
-      List.memP x (Interop.Adapters.ptrs_of_mem mem))
+    let mem = mk_mem (arg_of_sb stack::args) h0 in
+    ME.buffer_readable (as_vale_mem mem) (as_vale_buffer #bt x) <==>
+      List.memP x (ptrs_of_mem mem))
 
 val get_heap_mk_mem_reveal
   (#n:_)
   (args:IX64.arity_ok arg)
   (h0:HS.mem)
   (stack:IX64.stack_buffer n{mem_roots_p h0 (arg_of_sb stack::args)}) : Lemma
-  (let mem = Interop.Adapters.mk_mem (arg_of_sb stack::args) h0 in
-   Interop.Adapters.liveness_disjointness (arg_of_sb stack::args) h0;
-   MES.get_heap mem == IM.down_mem h0 IA.addrs (Interop.Adapters.args_b8 (arg_of_sb stack::args)))
+  (let mem = mk_mem (arg_of_sb stack::args) h0 in
+   liveness_disjointness (arg_of_sb stack::args) h0;
+   MES.get_heap (as_vale_mem mem) == I.down_mem mem)
 
 val buffer_as_seq_reveal
   (#n:_)
   (t:ME.base_typ)
-  (x:lowstar_buffer (ME.TBase t))
+  (x:buf_t t)
   (args:IX64.arity_ok arg)
   (h0:HS.mem)
   (stack:IX64.stack_buffer n{mem_roots_p h0 (arg_of_sb stack::args)}) : Lemma
   (let y = as_vale_buffer x in
-  let mem = Interop.Adapters.mk_mem (arg_of_sb stack::args) h0 in
-  assume (t <> ME.TUInt128); // TODO: UInt128
-  Seq.equal 
-    (LSig.nat_to_uint_seq_t t (ME.buffer_as_seq mem y))
+   let mem = mk_mem (arg_of_sb stack::args) h0 in
+   Seq.equal 
+    (LSig.nat_to_uint_seq_t t (ME.buffer_as_seq (as_vale_mem mem) y))
     (BV.as_seq h0 (BV.mk_buffer_view x (LSig.view_of_base_typ t))))
 
 val buffer_as_seq_reveal2
   (t:ME.base_typ)
-  (x:lowstar_buffer (ME.TBase t))
+  (x:buf_t t)
   (va_s:V.va_state) : Lemma
   (let y = as_vale_buffer x in
-  let h = Interop.Adapters.hs_of_mem va_s.VS.mem in
-  assume (t <> ME.TUInt128); // TODO: UInt128
-  Seq.equal 
+   let h = hs_of_mem (as_mem va_s.VS.mem) in
+   Seq.equal 
     (LSig.nat_to_uint_seq_t t (ME.buffer_as_seq va_s.VS.mem y))
     (BV.as_seq h (BV.mk_buffer_view x (LSig.view_of_base_typ t))))
 
 val buffer_addr_reveal
   (t:ME.base_typ)
-  (x:lowstar_buffer (ME.TBase t))
+  (x:buf_t t)
   (args:list arg)
   (h0:HS.mem{mem_roots_p h0 args}) : Lemma
-  (let mem = Interop.Adapters.mk_mem args h0 in
-  IA.addrs x == ME.buffer_addr (as_vale_buffer #(ME.TBase t) x) mem)
+  (let mem = mk_mem args h0 in
+   addrs_of_mem mem x == ME.buffer_addr (as_vale_buffer #t x) (as_vale_mem mem))
 
 val fuel_eq : squash (V.va_fuel == nat)
 
@@ -118,3 +110,11 @@ val decls_eval_code_reveal
   (f:V.va_fuel) : Lemma
   (requires (V.eval_code c va_s0 f va_s1))
   (ensures (VL.eval_code c va_s0 (coerce f) va_s1))
+
+val as_vale_buffer_disjoint (#t1 #t2:base_typ) (x:buf_t t1) (y:buf_t t2)
+   : Lemma (B.disjoint x y ==> ME.loc_disjoint (ME.loc_buffer (as_vale_buffer x)) (ME.loc_buffer (as_vale_buffer y)))
+           [SMTPat (ME.loc_disjoint (ME.loc_buffer (as_vale_buffer x)) (ME.loc_buffer (as_vale_buffer y)))]
+
+// module IB = Interop.Base
+// val valid_memtaint (mem:ME.mem) (ps:list b8{IB.list_disjoint_or_eq ps}) (ts:b8 -> GTot MS.taint)
+//   : Lemma (ME.valid_taint_bufs mem (IB.create_memtaint mem ps ts) ps ts)
